Path.v
@@ -5,6 +5,9 @@ Module PathTheories  (O: UsualOrderedType)(S: FSetInterface.Sfun O)(G: Graph O S
   Module G := Graph.
 
   Import G.
+
+(*There are a lot of essentially equivalent definitions of being a path in here. The only ones I use
+  are [path_list_ind] and [path_list_rev], which are also the most general, so we can get rid of the others*)
   
 
   Inductive path : graph -> vertex -> vertex -> Prop :=
@@ -52,28 +55,6 @@ Module PathTheories  (O: UsualOrderedType)(S: FSetInterface.Sfun O)(G: Graph O S
     - apply p_start. apply H.
     - eapply path_trans. apply p_start. apply H. apply IHpath'.
 Qed.
-
- (* Fixpoint path_list (g: graph) (u v : vertex) (l: list vertex) : bool :=
-    match l with
-    | nil => contains_edge g u v
-    | w :: t => contains_edge g u w && path_list g w v t
-    end.
-
-  Definition eq_bool (a b : O.t) :=
-    if O.eq_dec a b then true else false.
-
-  Lemma path_iff_list: forall g u v,
-    path g u v <-> exists l, path_list g u v l = true.
-  Proof.
-    intros. rewrite path_path'. split; intros.
-    - induction H.
-      + exists nil. simpl. apply H.
-      + destruct IHpath'. exists (w :: x). simpl. rewrite H. rewrite H1. reflexivity.
-    - destruct H. generalize dependent u. induction x; intros. 
-      + simpl in H. apply p_start'. apply H.
-      + simpl in H. rewrite andb_true_iff in H. destruct H.  eapply p_continue'.  apply H.
-        apply IHx. apply H0.
-  Qed.*)
 
   Inductive path_with: graph -> vertex -> vertex -> (vertex -> bool) -> Prop :=
     |  pw_start : forall g u v f,
@@ -126,20 +107,23 @@ Qed.
     - eapply p_continue. apply IHpath_with. apply H1.
   Qed.
 
-  Definition cycle_exists (g: graph) := exists v, path g v v.
- 
-  (*Is there a way to do this better without using law of excluded middle?*)
-  Definition acyclic (g: graph) := forall v, ~path g v v.
+  Definition acyclic (g: graph):= ~ exists v, path g v v.
+
+  Definition acyclic' (g: graph) := forall v, ~path g v v.
+
+  Lemma acyclic_equiv: forall g,
+    acyclic' g <-> acyclic g.
+  Proof.
+    intros. split; intros; unfold acyclic in *; unfold acyclic' in *. intro. destruct H0. apply (H x). apply H0.
+    intros. intro. apply H. exists v. apply H0.
+  Qed.
 
   Lemma alt_acyclic: forall g,
     acyclic g <-> (forall u v, path g u v -> u <> v).
   Proof.
     intros. split; intros.
-    - intro. subst. unfold acyclic in H. specialize (H v). contradiction.
-    - unfold acyclic. intros. intro. apply H in H0. contradiction.
+    - intro. subst. unfold acyclic in H. apply H. exists v. apply H0.
+    - unfold acyclic. intro. destruct H0. apply H in H0. contradiction.
   Qed.
-
-
-(*Let's see what we need later*)
 
 End PathTheories.
