Graph.v
@@ -4,7 +4,6 @@ Require Export Coq.FSets.FSetInterface.
 
 Module Type Graph (O: UsualOrderedType)(S: FSetInterface.Sfun O).
 
-
   Parameter graph: Type.
 
   Parameter empty : graph.
@@ -43,7 +42,6 @@ Module Type Graph (O: UsualOrderedType)(S: FSetInterface.Sfun O).
   Parameter contains_edge_2: forall g u v,
     contains_edge g u v = true ->
     contains_vertex g v = true.
-
 
   Parameter add_edge_1: forall g u v,
     contains_vertex g v = true ->
